improve logging2
transactions get an actual txid at runtime, and wait for that txid to
be committed to disk.  compared to the previous design, threads don't
wait longer than necessary now.  to do this, we introduced a commit
worker thread.

src/Examples/Logging2/ImplLog2.v
@@ -7,9 +7,11 @@ Definition log_start := 1.
 
 (* Memory addresses *)
 Definition log_lock := 0.
-Definition mem_lock := 1.
-Definition mem_count := 2.
-Definition mem_start := 3.
+Definition log_txn_next := 1.
+Definition mem_lock := 2.
+Definition mem_count := 3.
+Definition mem_txn_next := 4.
+Definition mem_start := 5.
 
 Definition log_data (pos : nat) :=
   log_start + pos.
@@ -50,20 +52,33 @@ Fixpoint read_mem_blocks (count : nat) (pos : nat) (res : list nat) :=
   )%proc.
 
 Definition disk_append :=
-  ( _ <- lock log_lock;
+  (
+    _ <- lock log_lock;
 
     disklen <- read_disk log_commit;
 
     _ <- lock mem_lock;
     memlen <- read_mem mem_count;
+    memtxns <- read_mem mem_txn_next;
     l <- read_mem_blocks (memlen-disklen) disklen nil;
     _ <- unlock mem_lock;
 
     _ <- write_blocks l disklen;
     _ <- write_disk log_commit memlen;
 
+    _ <- write_mem log_txn_next memtxns;
+
     _ <- unlock log_lock;
+
     Ret tt
+  )%proc.
+
+Definition disk_append_loop :=
+  (
+    Loop (R := unit) (fun _ =>
+      _ <- disk_append;
+      Ret (ContinueOutcome tt)
+    ) tt
   )%proc.
 
 Definition mem_append (l : list nat) :=
@@ -71,22 +86,36 @@ Definition mem_append (l : list nat) :=
     memlen <- read_mem mem_count;
     if gt_dec (memlen + length l) log_size then
       _ <- unlock mem_lock;
-      Ret false
+      Ret None
     else
+      memtxns <- read_mem mem_txn_next;
       _ <- write_mem_blocks l memlen;
       _ <- write_mem mem_count (memlen + length l);
+      _ <- write_mem mem_txn_next (memtxns+1);
       _ <- unlock mem_lock;
-      Ret true
+      Ret (Some memtxns)
+  )%proc.
+
+Definition disk_append_wait (memtxns : nat) :=
+  (
+    Loop (fun _ =>
+      logtxns <- read_mem log_txn_next;
+      if decide (memtxns < logtxns) then
+        Ret (DoneWithOutcome tt)
+      else
+        Ret (ContinueOutcome tt)
+    ) tt
   )%proc.
 
 Definition append (l : list nat) :=
   (
     ok <- mem_append l;
-    if ok then
-      _ <- disk_append;
+    match ok with
+    | None => Ret false
+    | Some memtxns =>
+      _ <- disk_append_wait memtxns;
       Ret true
-    else
-      Ret false
+    end
   )%proc.
 
 Fixpoint read_blocks (count : nat) (pos : nat) (res : list nat) :=
@@ -114,6 +143,7 @@ Definition impl : LayerImpl ExMach.Op Log2.Op :=
        match op with
        | Log2.Append l => append l
        | Log2.Read => read
+       | Log2.CommitWorker => disk_append_loop
        end;
      recover := Seq_Cons (recv) (Seq_Nil);
      (* init := Ret Initialized; *) |}.
